SStructTT.lean
@@ -15,3 +15,6 @@ import SStructTT.Static.Inversion
 import SStructTT.Static.Unique
 import SStructTT.Static.Preservation
 import SStructTT.Static.Progress
+
+import SStructTT.Dynamic.Context
+import SStructTT.Dynamic.Typed
